poST_utils/poST_expr_utils.thy
@@ -10,8 +10,6 @@ definition proc_status_is :: "proc_status \<Rightarrow> proc_status \<Rightarrow
   (proc_status.Error,proc_status.Error) \<Rightarrow> True |
   (proc_status.Stop,proc_status.Inactive) \<Rightarrow> True |
   (proc_status.Error,proc_status.Inactive) \<Rightarrow> True |
-  (proc_status.Timeout _, proc_status.Inactive) \<Rightarrow> True |
-  (proc_status.Timeout _, proc_status.Timeout _) \<Rightarrow> True |
   (_,_) \<Rightarrow> False)"
 declare proc_status_is_def [simp]
 
